\documentclass[convert={density=500}, border=2pt, varwidth=8in]{standalone}

\usepackage[utf8]{inputenc}
% \usepackage[htt]{hyphenat}
\usepackage{amsmath, amssymb, amsthm, thmtools, thm-restate, tikz, graphicx,
  hyperref, cleveref, comment, expl3, xparse, ebproof, enumitem,
  stmaryrd, verbatim, todonotes, xargs, tabularx, mathtools}

% https://tex.stackexchange.com/questions/188148/how-to-center-gathered-aligned-equations-in-enumerate-environment
\displaywidth=\textwidth
\displayindent=-\leftskip

\begin{document}
\begin{spreadlines}{2em}
\begin{gather*}
\textbf{Universal quantifier} \\
\begin{prooftree}
    \infer0{\mathtt{x} : A}
    \ellipsis{}{\mathtt{E} : B(x)}
    \infer1[$\forall I$]{\texttt{fun x => E} : \forall x : A, B(x)}
\end{prooftree}
~ \qquad
\begin{prooftree}
   \hypo{\mathtt{E_1} : \forall a : A, B(x)}
   \hypo{\mathtt{E_2} : A}
   \infer2[$\forall E$]{\mathtt{E_1 \,\, E_2} : B[x \mapsto E_2]} 
\end{prooftree}
\\ \textbf{Implication} \\
\begin{prooftree}
    \infer0{\mathtt{x} : A}
    \ellipsis{}{\mathtt{E} : B}
    \infer1[$\rightarrow I$]{\texttt{fun x => E} : A \rightarrow B}
\end{prooftree}
~ \qquad
\begin{prooftree}
   \hypo{\mathtt{E_1} : A \rightarrow B}
   \hypo{\mathtt{E_2} : A}
   \infer2[$\rightarrow E$]{\mathtt{E_1 \,\, E_2} : B} 
\end{prooftree}
\\ \textbf{Conjunction} \\
\begin{prooftree}
    \hypo{\mathtt{E_1} : A}
    \hypo{\mathtt{E_2} : B}
    \infer2[$\wedge I$]{\mathtt{(E_1, \, E_2)} : A \wedge B}
\end{prooftree}
~ \qquad
\begin{prooftree}
    \hypo{\mathtt{E} : A \wedge B}
    \infer1[$\wedge E_1$]{\mathtt{fst \,\, E} : A}
\end{prooftree}
~ \qquad
\begin{prooftree}
    \hypo{\mathtt{E} : A \wedge B}
    \infer1[$\wedge E_2$]{\mathtt{snd \,\, E} : B}
\end{prooftree}
\\ \textbf{Disjunction} \\
\begin{prooftree}
    \hypo{\mathtt{E} : A}
    \infer1[$\vee I_1$]{\mathtt{inl \,\, E} : A \vee B}
\end{prooftree}
~ \qquad
\begin{prooftree}
    \hypo{\mathtt{E} : B}
    \infer1[$\vee I_2$]{\mathtt{inr \,\, E} : A \vee B}
\end{prooftree}
\\
\begin{prooftree}
    \hypo{\mathtt{E} : A \vee B}
    \infer0{\mathtt{x} : A} \ellipsis{}{\mathtt{E_1} : C}
    \infer0{\mathtt{y} : B} \ellipsis{}{\mathtt{E_2} : C}
    \infer3[$\vee$ E]{
        \texttt{
            match E with
            | inl x => $\mathtt{E_1}$
            | inr y => $\mathtt{E_2}$
            end
        } : C
    }
\end{prooftree}
\\ \textbf{Existential quantifier} \\
\begin{prooftree}
    \hypo{\mathtt{E_1} : A}
    \hypo{\mathtt{E_2} : B[x \mapsto E_1]}
    \infer2[$\exists I$]{\mathtt{\{E_1, \, E_2\}} : \exists x : A, \, B(x)}
\end{prooftree}
~ \qquad
% https://tex.stackexchange.com/a/278156
\begin{prooftree}
    \hypo{\mathtt{E} : \exists x : A, \, B(x)}
    \infer0{\mathtt{x} : A}
    \infer0{\mathtt{y} : B(x)}
    \infer[no rule]2{}
    \ellipsis{}{\mathtt{E'} : C}
    \infer2[$\exists E$]{\texttt{let \{x, y\} := E in $\mathtt{E'}$} : C}
\end{prooftree}
\end{gather*}
\end{spreadlines}
\end{document}